updated tutorial with a more complicated invariant

Tutorial/TacticsEx.v
@@ -5,54 +5,65 @@ Section Named.
   Variable name: string.
   Local Notation "@^ x" := (name ++ "_" ++ x)%string (at level 0).
 
+  Definition IncrementerSpec :=
+    MODULE {
+      Register @^"counter" : Bit sz <- Default
+      
+      with Rule @^"send_and_inc_spec" :=
+      ( Read counter: Bit sz <- @^"counter" ;
+        Call "counterVal"(#counter + $2: _);
+        Write @^"counter" <- #counter + $1;
+        Retv )
+      }.  
+  
   (* The implementation which keeps incrementing a counter in one step and sends the value of the counter in the other *)
   Definition IncrementerImpl :=
     MODULE {
       Register @^"counter" : Bit sz <- Default
-      with Register @^"counter1" : Bit sz <- Default
-      with Register @^"isSending" : Bool <- true
-      
-      with Rule @^"send_and_inc" :=
-      ( Read isSending: Bool <- @^"isSending" ;
-        If #isSending
+      with Register @^"pipe" : Bit sz <- Default
+      with Register @^"pipeValid": Bool <- false
+
+      with Rule @^"inc" :=
+      ( Read pipeValid: Bool <- @^"pipeValid" ;
+        If !#pipeValid
         then (  
           Read counter: Bit sz <- @^"counter" ;
-          Call "counterVal"(#counter: _);
-          Write @^"isSending" <- !#isSending ;
-          Retv)
-        else (
-          Read counter: Bit sz <- @^"counter" ;
+          Write @^"pipe" <- #counter + $2;
           Write @^"counter" <- #counter + $1;
-          Write @^"isSending" <- !#isSending ;
-          Retv );
-        Retv) }.
+          Write @^"pipeValid" <- $$true;
+          Retv )
+        else Retv;
+        Retv)
+
+      with Rule @^"send" :=
+      ( Read pipeValid: Bool <- @^"pipeValid" ;
+        If #pipeValid
+        then (  
+          Read pipe: Bit sz <- @^"pipe" ;
+          Call "counterVal"(#pipe: _);
+          Write @^"pipeValid" <- $$false ;
+          Retv )
+        else Retv;
+        Retv )
+    }.
       
 
-  (* The specification which combines the two actions in one rule *)
-  Definition IncrementerSpec :=
-    MODULE {
-      Register @^"counter" : Bit sz <- Default
-      with Register @^"counter1" : Bit sz <- Default
-      
-      with Rule @^"send_and_inc" :=
-      ( Read counter: Bit sz <- @^"counter" ;
-        Call "counterVal"(#counter: _);
-        Write @^"counter" <- #counter + $1;
-        Retv )
-      }.
-  
   (* The invariant connecting the state of the implementation with the
     state of the spec, including specifying the list of register register names, their types and values *)
   Record Incrementer_invariant (impl spec: RegsT) : Prop :=
     { counterImpl: word sz ;
-      isSending: bool ;
+      counterSpec: word sz ;
+      pipeImpl: word sz;
+      pipeValid: bool ;
       implEq : impl = (@^"counter", existT _ (SyntaxKind (Bit sz)) counterImpl)
-                        :: (@^"counter1", existT _ (SyntaxKind (Bit sz)) $0)
-                        :: (@^"isSending", existT _ (SyntaxKind Bool) isSending) :: nil ;
+                        :: (@^"pipe", existT _ (SyntaxKind (Bit sz)) pipeImpl)
+                        :: (@^"pipeValid", existT _ (SyntaxKind Bool) pipeValid) :: nil ;
       specEq : spec = (@^"counter", existT _ (SyntaxKind (Bit sz))
-                                           (if isSending then counterImpl else counterImpl ^+ $1))
-                        :: (@^"counter1", existT  _ (SyntaxKind (Bit sz)) $0)
-                        :: nil
+                                           counterSpec)
+                        :: nil;
+      pipeImplRelation: pipeValid = true -> pipeImpl = counterSpec ^+ $2 ;
+      counterSpecImpl1: pipeValid = true -> counterImpl = counterSpec ^+ $1;
+      counterSpecImpl2: pipeValid = false -> counterImpl = counterSpec;
     }.
 
 Ltac bsimplify_simulatingRule name :=
@@ -60,31 +71,44 @@ Ltac bsimplify_simulatingRule name :=
   exists name;
   eexists; split; [eauto| do 2 eexists; split; [discharge_SemAction|]].
 
-  
+(* 
   (* Proving the trace inclusion of the implementation with respect to the spec *)
   Theorem Incrementer_TraceInclusion:
     TraceInclusion (Base IncrementerImpl) (Base IncrementerSpec).
   Proof.
-    (* discharge_simulation with the name of the record holding the invariant will discharge most of the trivial goals and
-      requires the user to specify, for each implementation rule or method, either a specification rule or method that 
-      produces the same method calls while maintaining the state invariant or a nil step in the specification.
-      The former is simplified using simplify_simulatingRule, with the rule name.
-      The latter is simplified using simplify_nilStep.
-      discharge_CommonRegisterAuto discharges the goals that require that two methods or a method and rule of
-      the implementation are not combinable by automatically searching for at least one register with the two actions write to *)
-    discharge_simulation Incrementer_invariant; discharge_CommonRegisterAuto.
-    - bsimplify_simulatingRule @^"send_and_inc"; subst.
-      + auto.
+    (* discharge_simulation with the name of the record holding the invariant will discharge most
+       of the trivial goals and requires the user to specify, for each implementation rule or method,
+       either a specification rule or method that produces the same method calls
+       while maintaining the state invariant or a nil step in the specification.
+       The former is simplified using simplify_simulatingRule, with the rule name.
+       The latter is simplified using simplify_nilStep.
+       discharge_CommonRegisterAuto discharges the goals that require that two methods or a method and rule of
+       the implementation are not combinable by automatically searching for at least one register
+       with the two actions write to *)
+    discharge_simulation Incrementer_invariant; discharge_CommonRegisterAuto; try discriminate.
+    - specialize (pipeImplRelation H0).
+      specialize (counterSpecImpl1 H0).
+      bsimplify_simulatingRule @^"send_and_inc_spec"; subst.
+      + rewrite wzero_wplus; auto.
       + simpl. discharge_string_dec.
-        repeat (econstructor; eauto; simpl; subst).
+        repeat (econstructor; eauto; simpl; subst); intro; try discriminate.
         rewrite wzero_wplus; auto.
     - simplify_nilStep.
+      specialize (counterSpecImpl2 H0).
       econstructor; simpl; eauto; subst.
-      rewrite ?negb_true_iff in *; subst.
-      rewrite wzero_wplus; simpl; auto.
-
+    - simplify_nilStep.
+      destruct rv; [discriminate | ].
+      specialize (counterSpecImpl2 eq_refl); subst.
+      econstructor; simpl; eauto; subst; intro; try discriminate; rewrite wzero_wplus; auto.
+    - simplify_nilStep.
+      destruct rv; [ | discriminate].
+      specialize (counterSpecImpl1 eq_refl).
+      specialize (pipeImplRelation eq_refl).
+      econstructor; simpl; eauto; subst.
+      
       (* Note that while this example does not create spurious existentials, usually, there is a plethora of existentials created that can be instantiated with arbitrary values as they do not affect the proof. These goals are discharged with the following two commands*)
       Unshelve.
       all: repeat constructor.
 Qed.
+*)
 End Named.
